fix time_restricted definition, rename to time_bounded
now defined in terms of input words, not arbitrary input tapes
both to stay in line with Hopcroft source definitions
move encoding section, as the definitions therein are used by time_bounded now

papers/116_stefan_rass/Complexity.thy
@@ -4,7 +4,7 @@ theory Complexity
 begin
 
 
-subsection\<open>Basic Measures\<close>
+subsection\<open>Basic Definitions\<close>
 
 text\<open>The tape size can not use the universal function \<^const>\<open>size\<close>,
   since for any pair \<^term>\<open>p = (a, b)\<close>, \<^term>\<open>size p = 1\<close>.\<close>
@@ -12,134 +12,14 @@ text\<open>The tape size can not use the universal function \<^const>\<open>size
 fun tape_size :: "tape \<Rightarrow> nat" \<comment> \<open>using \<open>fun\<close> since \<open>definition\<close> does not recognize patterns like \<^term>\<open>(l, r)\<close>\<close>
   where "tape_size (l, r) = length l + length r"
 
+text\<open>At the start of execution, the TM's head is over the first cell of the right tape.
+  That is, for \<^term>\<open>tp = (l, x # r)\<close>, the symbol under the head is \<open>x\<close>, or \<^term>\<open>read (snd tp)\<close>.
+  Additionally (through \<^const>\<open>read\<close>), the edge of the tape is interpreted as \<^const>\<open>Bk\<close>.\<close>
 
-subsubsection\<open>Time\<close>
-
-text\<open>The time restriction predicate is similar to \<^term>\<open>Hoare_halt\<close>,
-  but includes a maximum number of steps.
-  From Hopcroft, p287f:
-   "If for every input word of length n, M makes at most T(n) moves before
-    halting, then M is said to be a T(n) time-bounded Turing machine, or of time
-    complexity T(n). The language recognized by M is said to be of time complexity T(n)."
-
-   "[...] it is reasonable to assume that any time complexity function \<open>T(n)\<close> is
-    at least \<open>n + 1\<close>, for this is the time needed just to read the input and verify that the
-    end has been reached by reading the first blank.\<dagger> We thus make the convention
-    that "time complexity \<open>T(n)\<close>" means \<open>max (n + 1, \<lceil>T(n)\<rceil>])\<close>. For example, the value of
-    time complexity \<open>n log\<^sub>2n\<close> at \<open>m = 1\<close> is \<open>2\<close>, not \<open>0\<close>, and at \<open>n = 2\<close>, its value is \<open>3\<close>.
-
-    \<dagger> Note, however, that there are TM's that accept or reject without reading all their input.
-      We choose to eliminate them from consideration."\<close>
-
-abbreviation (input) tcomp :: "(nat \<Rightarrow> nat) \<Rightarrow> nat \<Rightarrow> nat"
-  where "tcomp T n \<equiv> max (n + 1) (T n)"
-
-definition time_restricted :: "(nat \<Rightarrow> nat) \<Rightarrow> TM \<Rightarrow> bool"
-  where "time_restricted T p \<equiv> \<forall>tp. \<exists>n.
-            n \<le> tcomp T (tape_size tp)
-          \<and> is_final (steps0 (1, tp) p n)"
-
-(* TODO (?) notation: \<open>p terminates_in_time T\<close> *)
-
-text\<open>\<open>time\<^sub>M(x)\<close> is the number of steps until the computation of \<open>M\<close> halts on input \<open>x\<close>,
-  or \<open>None\<close> if \<open>M\<close> does not halt on input \<open>x\<close>.\<close>
-
-definition time :: "TM \<Rightarrow> tape \<Rightarrow> nat option"
-  where "time M x \<equiv> (
-    if \<exists>n. is_final (steps0 (1, x) M n)
-      then Some (LEAST n. is_final (steps0 (1, x) M n))
-      else None
-    )"
+abbreviation head where "head tp \<equiv> read (snd tp)"
 
 
-text\<open>Notion of time-constructible from Hopcroft ch. 12.3, p. 299:
-  "A function T(n) is said to be time constructible if there exists a T(n) time-
-  bounded multitape Turing machine M such that for each n there exists some input
-  on which M actually makes T(n) moves."\<close>
-
-definition tconstr :: "(nat \<Rightarrow> nat) \<Rightarrow> bool"
-  where "tconstr T \<equiv> \<exists>M. \<forall>n. \<exists>w. time M ([], w) = Some (T n)"
-
-text\<open>Fully time-constructible, ibid.:
-  "We say that T(n) is fully time-constructible if there is a TM
-  that uses T(n) time on all inputs of length n."\<close>
-
-definition fully_tconstr :: "(nat \<Rightarrow> nat) \<Rightarrow> bool"
-  where "fully_tconstr T \<equiv> \<exists>M. \<forall>n w. length w = n \<longrightarrow> time M ([], w) = Some (T n)"
-
-lemma ftc_altdef: "fully_tconstr T \<longleftrightarrow> (\<exists>M. \<forall>w. time M ([], w) = Some (T (length w)))"
-  unfolding fully_tconstr_def by simp
-
-
-lemma time_restricted_altdef:
-  "time_restricted T p \<longleftrightarrow> (\<forall>tp. \<exists>n. time p tp = Some n \<and> n \<le> tcomp T (tape_size tp))"
-  unfolding time_restricted_def (* in order for the intros to work in direction "\<Longleftarrow>" *) Let_def
-proof (intro iffI allI exI conjI)
-  fix tp
-  let ?f = "\<lambda>n. is_final (steps0 (1, tp) p n)" let ?lf = "LEAST n. ?f n"
-  let ?tcompT = "\<lambda>tp. tcomp T (tape_size tp)"
-
-  assume (* time_restricted T p *) "\<forall>tp. \<exists>n \<le> ?tcompT tp. is_final (steps0 (1, tp) p n)"
-  then have n_ex: "\<exists>n. n \<le> ?tcompT tp \<and> ?f n" ..
-  then obtain n where "n \<le> ?tcompT tp" and "?f n" by blast
-
-  from n_ex have "\<exists>n. ?f n" by blast
-  then show "time p tp = Some ?lf" unfolding time_def by (rule if_P)
-  have "?lf \<le> n" using Least_le \<open>?f n\<close> .
-  also note \<open>n \<le> ?tcompT tp\<close>
-  finally show "?lf \<le> ?tcompT tp" .
-next
-  fix tp
-  let ?f = "\<lambda>n. is_final (steps0 (1, tp) p n)" let ?lf = "LEAST n. ?f n"
-  let ?tcompT = "\<lambda>tp. tcomp T (tape_size tp)"
-
-  assume "\<forall>tp. \<exists>n. time p tp = Some n \<and> n \<le> ?tcompT tp"
-  then obtain n where n_some: "time p tp = Some n" and n_le: "n \<le> ?tcompT tp" by blast
-
-  from n_some have "time p tp \<noteq> None" by (rule option.discI)
-  then have n_ex: "\<exists>n. ?f n" unfolding time_def by argo
-  with n_some have "?lf = n" unfolding time_def by simp
-
-  show "?f ?lf" using LeastI_ex n_ex .
-  show "?lf \<le> ?tcompT tp" unfolding \<open>?lf = n\<close> using n_le .
-qed
-
-corollary "time_restricted T p \<Longrightarrow> (\<forall>tp. the (time p tp) \<le> tcomp T (tape_size tp))"
-  unfolding time_restricted_altdef
-proof (intro allI, elim allE exE conjE)
-  fix tp n
-  assume some_n: "time p tp = Some n" and n_le: "n \<le> tcomp T (tape_size tp)"
-  from n_le show "the (time p tp) \<le> tcomp T (tape_size tp)" unfolding some_n option.sel .
-qed
-
-
-subsubsection\<open>Space\<close>
-
-(* implement adjustment similar to tcomp for space complexity. see Hopcroft p287 *)
-
-(* size of tape after M does n steps on input x *)
-abbreviation space0 where "space0 M x n \<equiv> let (_,tp) = steps0 (1, x) M n in tape_size tp"
-
-definition space_restricted :: "(nat \<Rightarrow> nat) \<Rightarrow> TM \<Rightarrow> bool"
-  where "space_restricted T M \<equiv> \<forall>x. \<forall>n. space0 M x n \<le> T(tape_size x)"
-
-definition space :: "TM \<Rightarrow> tape \<Rightarrow> nat"
-  where "space M x = Max {space0 M x n | n. n\<in>\<nat>}"
-
-
-lemma update_space_one: "tape_size (update a (l,r)) \<le> 1 + tape_size (l,r)"
-  by (induction a) simp_all
-lemma update_space_le: "tape_size (l,r) \<le> tape_size(update a (l,r))"
-  by (induction a) simp_all
-
-lemma step_space_mono: "space0 M x n \<le> space0 M x (Suc n)"
-  oops
-
-lemma tape_size_mono: "n \<le> m \<Longrightarrow> space0 M x n \<le> space0 M x m"
-  oops
-
-
-subsection\<open>Encoding Words\<close>
+subsubsection\<open>Encoding Words\<close>
 
 text\<open>Encoding binary words as TM tape cells: \<^term>\<open>True\<close> is encoded as \<^term>\<open>[Oc, Oc]\<close>
   and \<^term>\<open>False\<close> as \<^term>\<open>[Oc, Bk]\<close>.
@@ -177,25 +57,161 @@ proof (induction cs rule: is_encoded_word.induct)
 qed (* cases "cs = []", "cs = Bk # _", "cs = [_]" by *) simp_all
 
 
+text\<open>TM execution begins with the \<^const>\<open>head\<close> at the start of the input word.\<close>
+
+abbreviation input_tape ("<_>\<^sub>t\<^sub>p") where "<w>\<^sub>t\<^sub>p \<equiv> (([]::cell list), encode_word w)"
+
+\<comment> \<open>The following predicate is useful for Hoare statements.\<close>
+
+abbreviation input where "input w \<equiv> (\<lambda>tp. tp = <w>\<^sub>t\<^sub>p)"
+
+
+subsubsection\<open>Time\<close>
+
+text\<open>The time restriction predicate is similar to \<^term>\<open>Hoare_halt\<close>,
+  but includes a maximum number of steps.
+  From Hopcroft, p287f:
+   "If for every input word of length n, M makes at most T(n) moves before
+    halting, then M is said to be a T(n) time-bounded Turing machine, or of time
+    complexity T(n). The language recognized by M is said to be of time complexity T(n)."
+
+   "[...] it is reasonable to assume that any time complexity function \<open>T(n)\<close> is
+    at least \<open>n + 1\<close>, for this is the time needed just to read the input and verify that the
+    end has been reached by reading the first blank.\<dagger> We thus make the convention
+    that "time complexity \<open>T(n)\<close>" means \<open>max (n + 1, \<lceil>T(n)\<rceil>])\<close>. For example, the value of
+    time complexity \<open>n log\<^sub>2n\<close> at \<open>m = 1\<close> is \<open>2\<close>, not \<open>0\<close>, and at \<open>n = 2\<close>, its value is \<open>3\<close>.
+
+    \<dagger> Note, however, that there are TM's that accept or reject without reading all their input.
+      We choose to eliminate them from consideration."\<close>
+
+abbreviation (input) tcomp :: "(nat \<Rightarrow> nat) \<Rightarrow> nat \<Rightarrow> nat"
+  where "tcomp T n \<equiv> max (n + 1) (T n)"
+
+definition time_bounded :: "(nat \<Rightarrow> nat) \<Rightarrow> TM \<Rightarrow> bool"
+  where "time_bounded T M \<equiv> \<forall>w. \<exists>n.
+            n \<le> tcomp T (tape_size <w>\<^sub>t\<^sub>p)
+          \<and> is_final (steps0 (1, <w>\<^sub>t\<^sub>p) M n)"
+
+(* TODO (?) notation: \<open>p terminates_in_time T\<close> *)
+
+
+lemma time_bounded_altdef:
+  "time_bounded T M \<longleftrightarrow> (\<forall>w. is_final (steps0 (1, <w>\<^sub>t\<^sub>p) M (tcomp T (tape_size <w>\<^sub>t\<^sub>p))))"
+  unfolding time_bounded_def using is_final by blast
+
+lemma time_bounded_altdef':
+  "time_bounded T M \<Longrightarrow> is_final (steps0 (1, <w>\<^sub>t\<^sub>p) M (tcomp T (tape_size <w>\<^sub>t\<^sub>p)))"
+  using time_bounded_altdef by blast
+  
+
+text\<open>\<open>time\<^sub>M(x)\<close> is the number of steps until the computation of \<open>M\<close> halts on input \<open>x\<close>,
+  or \<open>None\<close> if \<open>M\<close> does not halt on input \<open>x\<close>.\<close>
+
+definition time :: "TM \<Rightarrow> tape \<Rightarrow> nat option"
+  where "time M x \<equiv> (
+    if \<exists>n. is_final (steps0 (1, x) M n)
+      then Some (LEAST n. is_final (steps0 (1, x) M n))
+      else None
+    )"
+
+
+text\<open>Notion of time-constructible from Hopcroft ch. 12.3, p. 299:
+  "A function T(n) is said to be time constructible if there exists a T(n) time-
+  bounded multitape Turing machine M such that for each n there exists some input
+  on which M actually makes T(n) moves."\<close>
+
+definition tconstr :: "(nat \<Rightarrow> nat) \<Rightarrow> bool"
+  where "tconstr T \<equiv> \<exists>M. \<forall>n. \<exists>w. time M ([], w) = Some (T n)"
+
+text\<open>Fully time-constructible, ibid.:
+  "We say that T(n) is fully time-constructible if there is a TM
+  that uses T(n) time on all inputs of length n."\<close>
+
+definition fully_tconstr :: "(nat \<Rightarrow> nat) \<Rightarrow> bool"
+  where "fully_tconstr T \<equiv> \<exists>M. \<forall>n w. length w = n \<longrightarrow> time M ([], w) = Some (T n)"
+
+lemma ftc_altdef: "fully_tconstr T \<longleftrightarrow> (\<exists>M. \<forall>w. time M ([], w) = Some (T (length w)))"
+  unfolding fully_tconstr_def by simp
+
+
+lemma time_bounded_altdef2:
+  "time_bounded T M \<longleftrightarrow> (\<forall>w. \<exists>n. time M <w>\<^sub>t\<^sub>p = Some n \<and> n \<le> tcomp T (tape_size <w>\<^sub>t\<^sub>p))"
+  unfolding time_bounded_def (* in order for the intros to work in direction "\<Longleftarrow>" *) Let_def
+proof (intro iffI allI exI conjI)
+  fix w
+  let ?f = "\<lambda>n. is_final (steps0 (1, <w>\<^sub>t\<^sub>p) M n)" let ?lf = "LEAST n. ?f n"
+  let ?tcompT = "\<lambda>tp. tcomp T (tape_size tp)"
+
+  assume (* time_bounded T p *) "\<forall>w. \<exists>n \<le> ?tcompT <w>\<^sub>t\<^sub>p. is_final (steps0 (1, <w>\<^sub>t\<^sub>p) M n)"
+  then have n_ex: "\<exists>n. n \<le> ?tcompT <w>\<^sub>t\<^sub>p \<and> ?f n" ..
+  then obtain n where "n \<le> ?tcompT <w>\<^sub>t\<^sub>p" and "?f n" by blast
+
+  from n_ex have "\<exists>n. ?f n" by blast
+  then show "time M <w>\<^sub>t\<^sub>p = Some ?lf" unfolding time_def by (rule if_P)
+  have "?lf \<le> n" using Least_le \<open>?f n\<close> .
+  also note \<open>n \<le> ?tcompT <w>\<^sub>t\<^sub>p\<close>
+  finally show "?lf \<le> ?tcompT <w>\<^sub>t\<^sub>p" .
+next
+  fix w
+  let ?f = "\<lambda>n. is_final (steps0 (1, <w>\<^sub>t\<^sub>p) M n)" let ?lf = "LEAST n. ?f n"
+  let ?tcompT = "\<lambda>w. tcomp T (tape_size <w>\<^sub>t\<^sub>p)"
+
+  assume "\<forall>w. \<exists>n. time M <w>\<^sub>t\<^sub>p = Some n \<and> n \<le> ?tcompT w"
+  then obtain n where n_some: "time M <w>\<^sub>t\<^sub>p = Some n" and n_le: "n \<le> ?tcompT w" by blast
+
+  from n_some have "time M <w>\<^sub>t\<^sub>p \<noteq> None" by (rule option.discI)
+  then have n_ex: "\<exists>n. ?f n" unfolding time_def by argo
+  with n_some have "?lf = n" unfolding time_def by simp
+
+  show "?f ?lf" using LeastI_ex n_ex .
+  show "?lf \<le> ?tcompT w" unfolding \<open>?lf = n\<close> using n_le .
+qed
+
+corollary "time_bounded T M \<Longrightarrow> the (time M <w>\<^sub>t\<^sub>p) \<le> tcomp T (tape_size <w>\<^sub>t\<^sub>p)"
+  unfolding time_bounded_altdef2
+proof (elim allE exE conjE)
+  fix tp n
+  assume some_n: "time M tp = Some n" and n_le: "n \<le> tcomp T (tape_size tp)"
+  from n_le show "the (time M tp) \<le> tcomp T (tape_size tp)" unfolding some_n option.sel .
+qed
+
+
+subsubsection\<open>Space\<close>
+
+(* implement adjustment similar to tcomp for space complexity. see Hopcroft p287 *)
+
+(* size of tape after M does n steps on input x *)
+abbreviation space0 where "space0 M x n \<equiv> let (_,tp) = steps0 (1, x) M n in tape_size tp"
+
+definition space_restricted :: "(nat \<Rightarrow> nat) \<Rightarrow> TM \<Rightarrow> bool"
+  where "space_restricted T M \<equiv> \<forall>x. \<forall>n. space0 M x n \<le> T(tape_size x)"
+
+definition space :: "TM \<Rightarrow> tape \<Rightarrow> nat"
+  where "space M x = Max {space0 M x n | n. n\<in>\<nat>}"
+
+
+lemma update_space_one: "tape_size (update a (l,r)) \<le> 1 + tape_size (l,r)"
+  by (induction a) simp_all
+lemma update_space_le: "tape_size (l,r) \<le> tape_size(update a (l,r))"
+  by (induction a) simp_all
+
+lemma step_space_mono: "space0 M x n \<le> space0 M x (Suc n)"
+  oops
+
+lemma tape_size_mono: "n \<le> m \<Longrightarrow> space0 M x n \<le> space0 M x m"
+  oops
+
+
 subsection\<open>Deciding Languages\<close>
 
 \<comment> \<open>Since \<open>L\<close> is a typical name for unspecified languages in the literature,
     the synonymous constructor \<^term>\<open>L\<close> of type \<^typ>\<open>action\<close> ("move head left") is hidden.\<close>
 hide_const (open) L
 
-abbreviation head where "head tp \<equiv> read (snd tp)"
-
 text\<open>A TM \<^term>\<open>p\<close> is considered to decide a language \<^term>\<open>L\<close>, iff for every possible word \<^term>\<open>w\<close>
   it correctly calculates language membership.
   That is, for \<^term>\<open>w \<in> L\<close> the computation results in \<^term>\<open>Oc\<close> under the TM head,
-  and for \<^term>\<open>w \<notin> L\<close> in \<^term>\<open>Bk\<close>.
-  The head is over the first cell of the right tape.
-  That is, for \<^term>\<open>tp = (l, x # r)\<close>, the symbol under the head is \<open>x\<close>, or \<^term>\<open>read (snd tp)\<close>.
-  Additionally (through \<^term>\<open>read\<close>), the edge of the tape is interpreted as \<^term>\<open>Bk\<close>.\<close>
-
-abbreviation input_tape ("<_>\<^sub>t\<^sub>p") where "<w>\<^sub>t\<^sub>p \<equiv> (([]::cell list), encode_word w)"
-
-abbreviation input where "input w \<equiv> (\<lambda>tp. tp = <w>\<^sub>t\<^sub>p)"
+  and for \<^term>\<open>w \<notin> L\<close> in \<^term>\<open>Bk\<close>.\<close>
 
 
 definition halts :: "TM \<Rightarrow> word \<Rightarrow> bool"
@@ -493,11 +509,11 @@ subsection\<open>DTIME\<close>
 
 text\<open>\<open>DTIME(T)\<close> is the set of languages decided by TMs in time \<open>T\<close> or less.\<close>
 definition DTIME :: "(nat \<Rightarrow> nat) \<Rightarrow> lang set"
-  where "DTIME T \<equiv> {L. \<exists>M. decides M L \<and> time_restricted T M}"
+  where "DTIME T \<equiv> {L. \<exists>M. decides M L \<and> time_bounded T M}"
 
 lemma in_dtimeI[intro]:
   assumes "decides M L"
-    and "time_restricted T M"
+    and "time_bounded T M"
   shows "L \<in> DTIME T"
   unfolding DTIME_def using assms by blast
 
@@ -505,12 +521,12 @@ lemma in_dtimeE[elim]:
   assumes "L \<in> DTIME T"
   obtains M
   where "decides M L"
-    and "time_restricted T M"
+    and "time_bounded T M"
   using assms unfolding DTIME_def by blast
 
 lemma in_dtimeE'[elim]:
   assumes "L \<in> DTIME T"
-  shows "\<exists>M. decides M L \<and> time_restricted T M"
+  shows "\<exists>M. decides M L \<and> time_bounded T M"
   using assms unfolding DTIME_def ..
 
 
@@ -519,17 +535,17 @@ lemma tcomp_mono: "(\<And>n. T n \<ge> t n) \<Longrightarrow> tcomp T n \<ge> tc
 lemma
   fixes T t
   assumes Tt: "\<And>n. T n \<ge> t n"
-    and tr: "time_restricted t M"
-  shows "time_restricted T M"
-  unfolding time_restricted_def
+    and tr: "time_bounded t M"
+  shows "time_bounded T M"
+  unfolding time_bounded_def
 proof (intro allI)
-  fix tp
-  from tr obtain n where n_tcomp: "n \<le> tcomp t (tape_size tp)"
-                     and final_n: "is_final (steps0 (1, tp) M n)"
-    unfolding time_restricted_def by blast
+  fix w
+  from tr obtain n where n_tcomp: "n \<le> tcomp t (tape_size <w>\<^sub>t\<^sub>p)"
+                     and final_n: "is_final (steps0 (1, <w>\<^sub>t\<^sub>p) M n)"
+    unfolding time_bounded_def by blast
 
-  from le_trans n_tcomp tcomp_mono Tt have "n \<le> tcomp T (tape_size tp)" .
-  with final_n show "\<exists>n\<le>tcomp T (tape_size tp). is_final (steps0 (1, tp) M n)" by blast
+  from le_trans n_tcomp tcomp_mono Tt have "n \<le> tcomp T (tape_size <w>\<^sub>t\<^sub>p)" .
+  with final_n show "\<exists>n\<le>tcomp T (tape_size <w>\<^sub>t\<^sub>p). is_final (steps0 (1, <w>\<^sub>t\<^sub>p) M n)" by blast
 qed
 
 
@@ -544,14 +560,14 @@ lemma simple_reduction:
     and "\<And>w. length (f\<^sub>R w) \<le> length w"
     and "\<And>w. Hoare_halt (input w) M\<^sub>R (input (f\<^sub>R w))"
     and "tm_wf0 M\<^sub>R"
-    and "time_restricted t\<^sub>R M\<^sub>R"
+    and "time_bounded t\<^sub>R M\<^sub>R"
     and "B \<in> DTIME(t)"
   defines "T \<equiv> \<lambda>n. t n + t\<^sub>R n"
   shows "A \<in> DTIME(T)"
 proof -
   from \<open>B \<in> DTIME t\<close> obtain M\<^sub>B
     where "decides M\<^sub>B B"
-      and "time_restricted t M\<^sub>B" ..
+      and "time_bounded t M\<^sub>B" ..
 
   define M where "M \<equiv> M\<^sub>R |+| M\<^sub>B"
 
@@ -566,33 +582,27 @@ proof -
     then have "{input w} M {\<lambda>tp. (head tp = Oc) = (w \<in> A)}" unfolding M_def \<open>w \<in> A \<longleftrightarrow> f\<^sub>R w \<in> B\<close> .
   }
   then have "decides M A" unfolding decides_altdef2' ..
-  moreover have "time_restricted T M"
+  moreover have "time_bounded T M"
   proof -
     fix w
+    define l where "l \<equiv> tape_size <w>\<^sub>t\<^sub>p"
       \<comment> \<open>Idea: Fix the input word \<^term>\<open>w\<close>.
-        We already know that the first machine \<^term>\<open>M\<^sub>R\<close> is time restricted
-        (@{thm \<open>time_restricted t\<^sub>R M\<^sub>R\<close>}),
-        such that its run-time will be no longer than \<^term>\<open>t\<^sub>R (tape_size <w>\<^sub>t\<^sub>p) = t\<^sub>R (2 * length w)\<close>
+        We already know that the first machine \<^term>\<open>M\<^sub>R\<close> is time bounded
+        (@{thm \<open>time_bounded t\<^sub>R M\<^sub>R\<close>}),
+        such that its run-time will be no longer than \<^term>\<open>t\<^sub>R l = t\<^sub>R (2 * length w)\<close>
         (times two due to the encoding \<^const>\<open>encode_word\<close>).
 
         We also know that it will result in the encoded corresponding input word
         with regards to \<open>B\<close> (@{thm \<open>\<And>w. {input w} M\<^sub>R {input (f\<^sub>R w)}\<close>}).
         Since the length of the corresponding input word is no longer
         than the length of the original input word \<^term>\<open>w\<close> (@{thm \<open>\<And>w. length (f\<^sub>R w) \<le> length w\<close>}),
-        and the second machine \<^term>\<open>M\<^sub>B\<close> is time restricted (@{thm \<open>time_restricted t M\<^sub>B\<close>}),
+        and the second machine \<^term>\<open>M\<^sub>B\<close> is time bounded (@{thm \<open>time_bounded t M\<^sub>B\<close>}),
         we may conclude that the run-time of \<^term>\<open>M \<equiv> M\<^sub>R |+| M\<^sub>B\<close> on the input \<^term>\<open><w>\<^sub>t\<^sub>p\<close>
-        is no longer than \<^term>\<open>T (tape_size <w>\<^sub>t\<^sub>p) \<equiv> t (tape_size <w>\<^sub>t\<^sub>p) + t\<^sub>R (tape_size <w>\<^sub>t\<^sub>p)\<close>.
+        is no longer than \<^term>\<open>T l \<equiv> t l + t\<^sub>R l\<close>.
 
-        Unfortunately, with the current definition of \<^const>\<open>time_restricted\<close>,
-        this does not imply \<^term>\<open>time_restricted T M\<close>.
-        For this to hold, the run-time must be restricted for all input-\<^emph>\<open>tapes\<close>,
-        and not only for all input-\<^emph>\<open>words\<close>.
-        Since not every tape encodes a word,
-        and the output length of the first TM \<^term>\<open>M\<^sub>R\<close> is only restricted for input words
-        (@{thm \<open>\<And>w. length (f\<^sub>R w) \<le> length w\<close>}),
-        the size of the intermediate tape is unrestricted,
-        such that even the time-restricted second machine \<^term>\<open>M\<^sub>B\<close> could run longer
-        than the afforded \<^term>\<open>t (tape_size <w>\<^sub>t\<^sub>p)\<close> steps.\<close>
+        \<^const>\<open>time_bounded\<close> is defined in terms of \<^const>\<open>tcomp\<close>, however,
+        which means that the resulting total run time \<^term>\<open>T l\<close> may be as large as
+        \<^term>\<open>tcomp t l + tcomp t\<^sub>R l \<equiv> max (l + 1) (t l) + max (l + 1) (t\<^sub>R l)\<close>.\<close>
 
     show ?thesis sorry
   qed
